Complexitylib/Classes/P.lean
@@ -11,6 +11,7 @@ public import Complexitylib.Classes.P.Composition
 public import Complexitylib.Classes.P.PairWithInput
 public import Complexitylib.Classes.P.Preimage
 public import Complexitylib.Classes.P.UnaryLength
+public import Complexitylib.Classes.P.Reverse
 public import Complexitylib.Classes.P.FinsetDomain
 public import Complexitylib.Classes.P.Cobham
 public import Complexitylib.Models.TuringMachine.Subroutines.CopyOutput
